Refactored functions from epoch into stake distribution

post-cip/formal-crypto/lean/src/Leioscrypto/Contexts.lean
@@ -1,5 +1,6 @@
 
 import Aesop
+import Leioscrypto.FaitAccompli
 import Leioscrypto.Registration
 import Leioscrypto.Types
 import Mathlib.Data.List.Defs
@@ -18,54 +19,15 @@ structure LeiosParameters where
   n_positive : 0 < n
 
 
-def StakeDistribution := List (PoolKeyHash × Coin)
-
-namespace StakeDistribution
-
-  def total_stake (stakes : StakeDistribution): Coin :=
-    (stakes.map Prod.snd).sum
-
-  def not_duplicated (stakes : StakeDistribution) : Prop :=
-    (stakes.map Prod.fst).Nodup
-
-  def have_stake (stakes : StakeDistribution) : Prop :=
-    ∀ stake ∈ stakes.map Prod.snd, stake > 0
-
-  def sorted_nonincreasing (stakes : StakeDistribution) : Prop :=
-    stakes.Pairwise $ fun ⟨ poolId₁ , stake₁ ⟩ ⟨ poolId₂ , stake₂ ⟩ ↦ stake₁ > stake₂ ∨ stake₁ = stake₂ ∧ poolId₁ > poolId₂
-
-end StakeDistribution
-
-
 structure Epoch where
   registry : Registry
   valid_registry : registry.IsValidRegistry
   number : Nat
-  pools : StakeDistribution
-  pools_not_duplicated : pools.not_duplicated
-  pools_have_stake : pools.have_stake
-  pools_sorted_nonincreasing : pools.sorted_nonincreasing
-  pools_valid_ids : ∀ p ∈ pools.map Prod.fst, p ∈ registry.map Registration.poolId
+  stakes : StakeDistribution
+  pools_valid_ids : ∀ p ∈ stakes.pools.map Prod.fst, p ∈ registry.map Registration.poolId
   slot_range : Slot × Slot
   slot_range_ordered : slot_range.fst ≤ slot_range.snd
   nonce : PraosNonce
-
-namespace Epoch
-
-  def lookup (epoch : Epoch) (i : Nat) (h : i < epoch.pools.length) : PoolKeyHash × Coin :=
-    epoch.pools.get ⟨ i, h ⟩
-
-  def lookupPoolId (epoch : Epoch) (i : Nat) (h : i < epoch.pools.length) : PoolKeyHash :=
-    Prod.fst $ epoch.pools.get ⟨ i , h ⟩
-
-  theorem poolId_in_pools (epoch : Epoch) (i : Nat) (h : i < epoch.pools.length) : lookupPoolId epoch i h ∈ epoch.pools.map Prod.fst :=
-    by
-      let poolId := epoch.lookupPoolId i h
-      rw [lookupPoolId]
-      apply List.mem_map_of_mem
-      apply List.get_mem
-
-end Epoch
 
 
 structure Election where
