post-cip/formal-crypto/lean/src/Leioscrypto/FaitAccompli.lean
@@ -1,0 +1,51 @@
+
+import Leioscrypto.Types
+
+
+namespace Leioscrypto
+
+
+structure StakeDistribution where
+  pools : List (PoolKeyHash × Coin)
+  not_duplicated : (pools.map Prod.fst).Nodup
+  have_stake : ∀ stake ∈ pools.map Prod.snd, stake > 0
+  sorted_nonincreasing : pools.Pairwise $ fun ⟨ poolId₁ , stake₁ ⟩ ⟨ poolId₂ , stake₂ ⟩ ↦ stake₁ > stake₂ ∨ stake₁ = stake₂ ∧ poolId₁ > poolId₂
+
+namespace StakeDistribution
+
+  def lookup (stakes : StakeDistribution) (i : Nat) (h : i < stakes.pools.length) : PoolKeyHash × Coin :=
+    stakes.pools.get ⟨ i, h ⟩
+
+  def lookupPoolId (stakes : StakeDistribution) (i : Nat) (h : i < stakes.pools.length) : PoolKeyHash :=
+    Prod.fst $ stakes.pools.get ⟨ i , h ⟩
+
+  theorem poolId_in_pools (stakes : StakeDistribution) (i : Nat) (h : i < stakes.pools.length) : lookupPoolId stakes i h ∈ stakes.pools.map Prod.fst :=
+    by
+      let poolId := stakes.lookupPoolId i h
+      rw [lookupPoolId]
+      apply List.mem_map_of_mem
+      apply List.get_mem
+
+
+  def total (stakes : StakeDistribution): Coin :=
+    (stakes.pools.map Prod.snd).sum
+
+  def remaining (stakes : StakeDistribution) : List Coin :=
+    Prod.fst
+      $ stakes.pools.foldr (init := ([], 0))
+        fun ⟨ _ , stake ⟩ (acc, previousTotal) =>
+          let newTotal := stake + previousTotal
+          (newTotal :: acc, newTotal)
+
+end StakeDistribution
+
+
+/-
+def persistentSeatCount (n : Nat) (stakes : StakeDistribution) : Nat :=
+  let test (i : Nat) (S : Nat) (ρ : Nat) : Bool :=
+    (n - i + 1) * (ρ - S)^2 ≥ (n - i) * ρ^2
+  let ρs := stakes.remaining
+  sorry
+-/
+
+end Leioscrypto
